src/Std/Sat/AIG/DetectGates.lean
@@ -1,0 +1,123 @@
+/-
+Copyright (c) 2026 Lean FRO, LLC. All rights reserved.
+Released under Apache 2.0 license as described in the file LICENSE.
+Authors: George Rennie
+-/
+module
+
+prelude
+public import Std.Sat.AIG.Lemmas
+import Init.Omega
+
+@[expose] public section
+
+/-!
+This module contains functions to detect compound logic gates represented by sub-graphs of the `AIG`.
+-/
+
+namespace Std
+namespace Sat
+
+namespace AIG
+
+variable {α : Type} [Hashable α] [DecidableEq α]
+
+/--
+Try to detect an XOR/XNOR gate rooted at the given entrypoint, returning a pair of `Refs` with
+the same semantics as `entry` when XORed.
+
+This can detect XOR/XNOR gates represented in the two-level form `¬(a ∧ b) ∧ ¬(¬a ∧ ¬b)` up to
+permutation of inputs and negation of inputs and output.
+-/
+def detectXor (entry : Entrypoint α) : Option entry.aig.BinaryInput := do
+  have := entry.ref.hgate
+  -- Match root = (l ∧ r)
+  let (eq:=hroot) .gate l r := entry.aig.decls[entry.ref.gate] | none
+  have := entry.aig.hdag entry.ref.hgate hroot
+
+  -- We expect the structure to be a (potentially inverted) conjunction of disjunctions so l/r
+  -- must be inverted
+  let true := l.invert && r.invert | none
+
+  -- Match l = (l0 ∧ l1)
+  let (eq:=hl) .gate l0 l1 := entry.aig.decls[l.gate] | none
+  have := entry.aig.hdag (by omega) hl
+
+  -- Match r = (r0 ∧ r1)
+  let (eq:=hr) .gate r0 r1 := entry.aig.decls[r.gate] | none
+  have := entry.aig.hdag (by omega) hr
+
+  -- l and r must have the same inputs with opposite inversions to be an xor. We consider both
+  -- permutations of l/r inputs with one another.
+  if (l0 = r0.flip true ∧ l1 = r1.flip true) ∨ (l1 = r0.flip true ∧ l0 = r1.flip true) then
+    -- If the root is uninverted, the gate represents `l0 xor l1`, otherwise it represents
+    -- `l0 xnor l1` = `l0 xor ¬l1`.
+    let lhs := ⟨l0.gate, l0.invert, by omega⟩
+    let rhs := (⟨l1.gate, l1.invert, by omega⟩ : Ref entry.aig).flip entry.ref.invert
+    some ⟨lhs, rhs⟩
+  else
+    none
+
+variable {assign}
+
+theorem denote_detectXor {entry : Entrypoint α} {fi : entry.aig.BinaryInput} (heq : detectXor entry = some fi) :
+    ⟦entry, assign⟧ = (⟦entry.aig, fi.lhs, assign⟧ ^^ ⟦entry.aig, fi.rhs, assign⟧) := by
+  simp only [detectXor] at heq
+  split at heq; (all_goals try contradiction); next l r hroot =>
+  split at heq; (all_goals try contradiction); next hinvert =>
+  split at heq; (all_goals try contradiction); next l0 l1 hl =>
+  split at heq; (all_goals try contradiction); next r0 r1 hr =>
+  split at heq; (all_goals try contradiction); next hmatch =>
+  · simp at hinvert
+    rw [denote_idx_gate hroot, hinvert.left, hinvert.right, denote_idx_gate hl, denote_idx_gate hr]
+    simp only [Option.some.injEq] at heq
+    rcases hmatch with ⟨hl0, hl1⟩ | ⟨hl0, hl1⟩
+    · have {a b : Bool} : ((a || b) && (!a || !b)) = (a ^^ b) := by cases a <;> cases b <;> decide
+      simp only [hl0, Fanin.gate_flip, Fanin.invert_flip, Bool.bne_true, denote_not_invert, hl1,
+        Bool.not_and, Bool.not_not, this, ← heq]
+      <;> cases r0.invert
+      <;> cases r1.invert
+      <;> cases entry.ref.invert
+      <;> simp
+    · have {a b : Bool} : ((a || b) && (!b || !a)) = (a ^^ b) := by cases a <;> cases b <;> decide
+      simp only [hl0, Fanin.gate_flip, Fanin.invert_flip, Bool.bne_true, denote_not_invert, hl1,
+        Bool.not_and, Bool.not_not, this, ← heq]
+      <;> cases r0.invert
+      <;> cases r1.invert
+      <;> cases entry.ref.invert
+      <;> simp
+
+theorem detectXor_lhs_lt {entry : Entrypoint α} {fi : entry.aig.BinaryInput} (heq : detectXor entry = some fi) :
+    fi.lhs.gate < entry.ref.gate := by
+  simp only [detectXor] at heq
+  split at heq; (all_goals try contradiction); next l r hroot =>
+  split at heq; (all_goals try contradiction); next hinvert =>
+  split at heq; (all_goals try contradiction); next l0 l1 hl =>
+  split at heq; (all_goals try contradiction); next r0 r1 hr =>
+  split at heq; (all_goals try contradiction); next hmatch =>
+  have := entry.ref.hgate
+  have := entry.aig.hdag (by omega) hroot
+  have := entry.aig.hdag (by omega) hl
+  rw [Option.some.injEq] at heq
+  simp only [← heq]
+  omega
+
+theorem detectXor_rhs_lt {entry : Entrypoint α} {fi : entry.aig.BinaryInput} (heq : detectXor entry = some fi) :
+    fi.rhs.gate < entry.ref.gate := by
+  simp only [detectXor] at heq
+  split at heq; (all_goals try contradiction); next l r hroot =>
+  split at heq; (all_goals try contradiction); next hinvert =>
+  split at heq; (all_goals try contradiction); next l0 l1 hl =>
+  split at heq; (all_goals try contradiction); next r0 r1 hr =>
+  split at heq; (all_goals try contradiction); next hmatch =>
+  have := entry.ref.hgate
+  have := entry.aig.hdag (by omega) hroot
+  have := entry.aig.hdag (by omega) hl
+  rw [Option.some.injEq] at heq
+  simp only [← heq, Ref.gate_flip]
+  omega
+
+end AIG
+
+end Sat
+end Std
